new file:   c/cs/myecho.c 	new file:   c/cs/syscall/getenv.c 	new file:   c/cs/syscall/setenv.c 	modified:   coq/cat/Setoids.v 	modified:   coq/sf/Imp_code.v 	modified:   coq/sf/Makefile 	modified:   coq/sf/eval.v 	modified:   coq/sf/test_eval.v 	modified:   haskell/wiwik/Quasiquotation.hs 	new file:   haskell/wiwik/Quasiquote.hs 	new file:   haskell/wiwik/Quasiquote2.hs 	new file:   haskell/wiwik/TemplateHaskell.hs 	modified:   test.sh

c/cs/myecho.c
@@ -1,0 +1,26 @@
+#include <stdio.h>
+
+
+int main(int argc, const char *argv[], const char *envp[])
+{
+    printf("\n\n%d arguments were passed to the program\n", argc);
+
+    int i;
+    for(i = 0; i < argc; ++i)
+    {
+        printf("argv[%d] = %s\n", i, argv[i]);
+    }
+
+
+    printf("\n\nEnvironment variables are as follows:\n");
+    i = 0;
+    while (envp[i] != NULL) {
+        printf("envp[%d] = %s\n", i, envp[i]);
+        ++i;
+    }
+
+
+
+    return 0;
+
+}
