c/cs/syscall/getenv.c
@@ -1,0 +1,16 @@
+#include <stdio.h>
+#include <stdlib.h>
+
+int main() {
+
+    char *p;
+
+    const char* NAME = "VIM";
+
+
+    p = getenv(NAME);
+
+    printf("%s = %s\n", NAME, p);
+
+    return 0;
+}
