c/cs/syscall/setenv.c
@@ -1,0 +1,33 @@
+#include <stdio.h>
+#include <stdlib.h>
+
+
+int main(int argc, const char *argv[], const char *envp[])
+{
+
+    char *p = getenv("A");
+
+    if(p != NULL)
+        printf("The environment variable A is set to %s\n", p);
+    else
+        printf("The environment variable A is not yet set\n");
+
+
+    printf("Now setting A to the value /usr/share/vim\n");
+
+    if(setenv("A","/usr/share/vim",1) == 0)
+        printf("The environment variable A is now set to %s\n", getenv("A"));
+    else
+        printf("The setting of A was unsuccessful\n");
+
+    printf("\n\nEnvironment variables are as follows:\n");
+    int i = 0;
+    while (envp[i] != NULL) {
+        printf("envp[%d] = %s\n", i, envp[i]);
+        ++i;
+    }
+
+
+    return 0;
+
+}
