haskell/wiwik/Quasiquote.hs
@@ -1,0 +1,14 @@
+{-# LANGUAGE QuasiQuotes #-}
+
+import Quasiquotation
+
+
+a :: Expr
+a = [calc|true|]
+
+b :: Expr
+b = [calc|succ (succ 0)|]
+
+
+c :: Expr
+c = [calc|pred (succ 0)|]
