haskell/wiwik/Quasiquote2.hs
@@ -1,0 +1,2 @@
+import qualified Language.C.Syntax as C
+--import qualified Language.C.Quote.CUDA as Cuda
