haskell/wiwik/TemplateHaskell.hs
@@ -1,0 +1,49 @@
+{-# LANGUAGE QuasiQuotes #-}
+{-# LANGUAGE TemplateHaskell #-}
+
+import Language.Haskell.TH
+
+-- Expression 
+ex1 :: IO Exp   
+ex1 = runQ [e| \x -> x |]
+-- LamE [VarP x_0] (VarE x_0)
+
+ex1' :: IO Exp
+ex1' = runQ [| \x -> x |]       -- 'e' optional
+-- LamE [VarP x_0] (VarE x_0)
+
+-- Declaration
+ex2 :: IO [Dec] 
+ex2 = runQ [d| data Nat = Z | S Nat |]
+-- [DataD [] Nat_0 [] Nothing [NormalC Z_1 [],NormalC S_2 [(Bang NoSourceUnpackedness NoSourceStrictness,ConT Nat_0)]] []]
+
+data Nat' = Z' | S' Nat'
+
+-- Pattern
+ex3 :: IO Pat
+ex3 = runQ [p| S' (S' Z') |]
+-- ConP Main.S' [ConP Main.S' [ConP Main.Z' []]]
+
+-- Type
+ex4 :: IO Type
+ex4 = runQ [t| Int -> [Int] |]
+-- AppT (AppT ArrowT (ConT GHC.Types.Int)) (AppT ListT (ConT GHC.Types.Int))
+
+ex5 = $(runQ [| \x -> x |]) 3
+-- 3
+
+-- builds the function (f = \(a,b) -> a)
+f :: Q [Dec]
+f = do
+    let f = mkName "f"
+    a <- newName "a"
+    b <- newName "b"
+    return [ FunD f [ Clause [ TupP [VarP a, VarP b]] (NormalB (VarE a)) [] ] ]
+
+ex6 :: IO [Dec]
+ex6 = runQ f
+-- [FunD f [Clause [TupP [VarP a_0,VarP b_1]] (NormalB (VarE a_0)) []]]
+
+
+
+
