coq/sf/Imp_code.v
@@ -19,7 +19,27 @@ Definition Dec_x_z : com :=
     z ::= AMinus (AKey z) (ANum 1);;
     x ::= AMinus (AKey x) (ANum 1).
 
+Definition subtract_slowly : com :=
+    WHILE BNot (BEq (AKey x) (ANum 0)) DO
+        Dec_x_z
+    END.
 
+Definition minus_5_4 : com :=
+    x ::= ANum 3;;
+    z ::= ANum 5;;
+    subtract_slowly.
+
+Definition loop : com :=
+    WHILE BTrue DO
+        SKIP
+    END.
+
+Definition pup_to_n : com :=
+    y ::= ANum 0;;
+    WHILE BNot (BEq (AKey x) (ANum 0)) DO
+        y ::= APlus  (AKey y) (AKey x) ;;
+        x ::= AMinus (AKey x) (ANum 1)
+    END.
 
 
  
