coq/sf/eval.v
@@ -2,6 +2,7 @@ Require Import bool.
 Require Import nat.
 Require Import syntax.
 Require Import state.
+Require Import dictionary.
 
 
 Fixpoint aeval (env:State) (a:aexp) : nat :=
@@ -24,4 +25,30 @@ Fixpoint beval (env:State) (b:bexp) : bool :=
     | BAnd b1 b2    => andb (beval env b1) (beval env b2)
     end.
 
+Fixpoint ceval_fun_no_while (env:State) (c:com) : State :=
+    match c with
+    | SKIP                      => env
+    | x ::= a1                  => t_update env x (aeval env a1)
+    | c1 ;; c2                  => let env' := ceval_fun_no_while env c1 
+                                   in ceval_fun_no_while env' c2
+    | IFB b THEN c1 ELSE c2 FI  => if (beval env b)
+                                   then ceval_fun_no_while env c1
+                                   else ceval_fun_no_while env c2 
+    | WHILE b DO c END          => env
+    end.
 
+
+Inductive ceval : com -> State -> State -> Prop :=
+| E_Skip     : forall e, ceval SKIP e e
+| E_Ass      : forall e a n x, aeval e a = n -> ceval (x ::= a) e (t_update e x n)
+| E_Seq      : forall e e' e'' c1 c2, ceval c1 e e' -> ceval c2 e' e'' ->
+                ceval (c1 ;; c2) e e''
+| E_IfTrue   : forall e e' b c1 c2, beval e b = true -> ceval c1 e e' ->
+                ceval (IFB b THEN c1 ELSE c2 FI) e e'
+| E_IfFalse  : forall e e' b c1 c2, beval e b = false -> ceval c2 e e' ->
+                ceval (IFB b THEN c1 ELSE c2 FI) e e'
+| E_WhileEnd : forall e b c, beval e b = false -> ceval (WHILE b DO c END) e e
+| E_WhileLoop: forall e e' e'' b c, beval e b = true -> ceval c e e' ->
+                ceval (WHILE b DO c END) e' e'' -> 
+                ceval (WHILE b DO c END) e  e''
+.
