coq/sf/test_eval.v
@@ -3,6 +3,8 @@ Require Import nat.
 Require Import syntax.
 Require Import eval.
 Require Import state.
+Require Import dictionary.
+Require Import Imp_code.
 
 Example test_aeval0 : forall (env:State), aeval env (ANum 17) = 17.
 Proof. reflexivity. Qed.
@@ -18,3 +20,51 @@ Proof. reflexivity. Qed.
 
 Example test_aeval3 : forall (env:State), aeval env (AMult (ANum 4) (ANum 5)) = 20.
 Proof. reflexivity. Qed.
+
+Example test_ceval1 : ceval (
+    x ::= ANum 2;;
+    IFB BLe (AKey x) (ANum 1)
+        THEN y ::= ANum 3
+        ELSE z ::= ANum 4
+    FI) 
+    emptyState
+    (t_update (t_update emptyState x 2) z 4).
+Proof.
+    apply E_Seq with (e' := t_update emptyState x 2).
+    - apply E_Ass. reflexivity.
+    - apply E_IfFalse.
+        + reflexivity.
+        + apply E_Ass. reflexivity.
+Qed.
+
+(*
+Theorem test_ceval2 : ceval pup_to_n 
+    (t_update emptyState x 3)
+    (t_update
+        (t_update
+            (t_update 
+                (t_update
+                    (t_update 
+                        (t_update 
+                            (t_update 
+                                (t_update 
+                                    emptyState 
+                                    x 3)  y 0) y 3) x 2) y 5) x 1) y 6) x 0).
+Proof.
+    remember (t_update emptyState x 3) as e0 eqn:E0.
+    remember (t_update e0 y 0) as e1 eqn:E1.
+    remember (t_update e1 y 3) as e2 eqn:E2.
+    remember (t_update e2 x 2) as e3 eqn:E3.
+    remember (t_update e3 y 5) as e4 eqn:E4.
+    remember (t_update e4 x 1) as e5 eqn:E5.
+    remember (t_update e5 y 6) as e6 eqn:E6.
+    remember (t_update e6 x 0) as e7 eqn:E7. 
+    apply E_Seq with (e':=e1).
+        - rewrite E1. apply E_Ass. reflexivity.
+        - apply E_WhileLoop with (e':=e2).
+            + rewrite E1. rewrite E0. reflexivity.  
+            +
+            
+
+Show.
+*)
